valid_ptr: make fractional
Progress, Pointers: allocation and object IDs + fractional validity

There's too much boilerplate in these fractional instances --- for a moment I
thought I had screwed up something.

Problem: the module setup isn't the right one.
(cherry picked from commit 0e881afe33ea48a6fe7dcedd2c9746c3c44ad483)

valid_ptr nullptr is Persistent, and only accidentally Fractional

Reorder instances accordingly.

WIP identity_forget is a fancy update

theories/lang/cpp/logic/pred.v
@@ -13,6 +13,7 @@
  *)
 From Coq.Classes Require Import
      RelationClasses Morphisms.
+From stdpp Require Import namespaces strings.
 
 From iris.base_logic.lib Require Export iprop.
 Require Import iris.bi.monpred.
@@ -27,6 +28,8 @@ Export ChargeNotation.
 From bedrock.lang.cpp Require Import ast semantics.
 
 Set Default Proof Using "Type".
+
+Definition logicN : namespace := nroot .@ "bedrock.logic".
 
 Module Type CPP_LOGIC_CLASS_BASE.
   Parameter cppG : gFunctors -> Type.
@@ -106,14 +109,16 @@ Module Type CPP_LOGIC (Import CC : CPP_LOGIC_CLASS) (Import PTR : PTR_API).
     Context `{Σ : cpp_logic}.
 
     (* valid pointers allow for accessing one past the end of a structure/array *)
-    Parameter valid_ptr : ptr -> mpred.
+    Parameter valid_ptr : ptr -> Qp -> mpred.
 
-    Axiom valid_ptr_persistent : forall p, Persistent (valid_ptr p).
-    Axiom valid_ptr_affine : forall p, Affine (valid_ptr p).
-    Axiom valid_ptr_timeless : forall p, Timeless (valid_ptr p).
-    Global Existing Instances valid_ptr_persistent valid_ptr_affine valid_ptr_timeless.
+    Axiom valid_ptr_fractional : forall p, Fractional (valid_ptr p).
+    Axiom valid_ptr_affine : forall p q, Affine (valid_ptr p q).
+    Axiom valid_ptr_timeless : forall p q, Timeless (valid_ptr p q).
+    Global Existing Instances valid_ptr_fractional valid_ptr_affine valid_ptr_timeless.
 
-    Axiom valid_ptr_nullptr : |-- valid_ptr nullptr.
+    (* The fraction is not relevant for nullptr. *)
+    Axiom valid_ptr_nullptr : forall q, |-- valid_ptr nullptr q.
+    Axiom valid_ptr_nullptr_persistent : forall q, Persistent (valid_ptr nullptr q).
 
     (**
     Typed points-to predicate. Fact [tptsto t q p v] asserts the following things:
@@ -174,6 +179,7 @@ Module Type CPP_LOGIC (Import CC : CPP_LOGIC_CLASS) (Import PTR : PTR_API).
         compilers can use the ownership here to represent dynamic dispatch
         tables.
      *)
+    (* XXX reconceive this to track "object creation" in the abstract machine. *)
     Parameter identity : forall {σ : genv}
         (this : globname) (most_derived : option globname),
         Qp -> ptr -> mpred.
@@ -181,9 +187,12 @@ Module Type CPP_LOGIC (Import CC : CPP_LOGIC_CLASS) (Import PTR : PTR_API).
 
     (** this allows you to forget an object identity, necessary for doing
         placement [new] over an existing object.
+        XXX in fact, we should talk about types, and go from/to "array of
+        bytes" to "fancier objects".
      *)
     Axiom identity_forget : forall σ mdc this p,
-        @identity σ this (Some mdc) 1 p |-- @identity σ this None 1 p.
+        @identity σ this (Some mdc) 1 p
+        |-- |={↑logicN}=> @identity σ this None 1 p.
 
     (** the pointer points to the code
 
